Seccompjit.v: return error when no trailing ret

Seccompjit.v
@@ -9,53 +9,43 @@ Require Import Seccomp.
 
 Parameter seccomp_memwords: Z.
 
-Record state: Type := mkstate {
-  st_code: RTL.code;
-  st_ep: node;
-  st_map: ZMap.t node
-}.
+Inductive state: Type :=
+  | empty_state: state
+  | code_state:   (* pcmap maps Seccomp.v pc's to RTL.code ep's *)
+    forall (code: RTL.code) (entry: node) (pcmap: PTree.t node), state.
 
-Record fnmap: Type := mkfnmap {
-  fn: RTL.function;
-  map: ZMap.t node
-}.
+Definition next_ep (s: state) :=
+  match s with
+  | empty_state => 1%positive
+  | code_state _ ep _ => (Psucc ep)
+  end.
 
-Inductive state_incr: state -> state -> Prop :=
-  state_incr_intro:
-    forall (s1 s2: state),
-    Ple s1.(st_ep) s2.(st_ep) ->
-    (forall pc,
-      s1.(st_code)!pc = None \/ s2.(st_code)!pc = s1.(st_code)!pc) ->
-    state_incr s1 s2.
+Definition st_code (s: state) :=
+  match s with
+  | empty_state => PTree.empty RTL.instruction
+  | code_state c _ _ => c
+  end.
 
-Lemma state_incr_refl:
-  forall s, state_incr s s.
-Proof.
-  intros.
-  apply state_incr_intro.
-  apply Ple_refl.
-  intros; auto.
-Qed.
+Definition st_map (s: state) :=
+  match s with
+  | empty_state => PTree.empty node
+  | code_state _ _ m => m
+  end.
 
-Lemma state_incr_trans:
-  forall s1 s2 s3, state_incr s1 s2 -> state_incr s2 s3 -> state_incr s1 s3.
-Proof.
-  intros.
-  inv H; inv H0.
-  apply state_incr_intro.
-  apply Ple_trans with s2.(st_ep); assumption.
+Definition st_ep (s: state) : res node :=
+  match s with
+  | empty_state => Error (msg "No entry point for empty function")
+  | code_state _ ep _ => OK ep
+  end.
 
-  intros.
-  generalize (H2 pc) (H3 pc).
-  intuition congruence.
-Qed.
-
-Definition add_instr (instr: RTL.instruction) (st: state) : state :=
-  let n := Psucc st.(st_ep) in
-  mkstate (PTree.set n instr st.(st_code)) n st.(st_map).
-
-Definition add_map (pc: Z) (st: state) : state :=
-  mkstate st.(st_code) st.(st_ep) (ZMap.set pc st.(st_ep) st.(st_map)).
+Definition add_instr (instr: RTL.instruction) (st: state)
+                     (opc: option positive) : state :=
+  let new_ep := next_ep st in
+  let new_map := match opc with
+    | None => st_map st
+    | Some pc => (PTree.set pc new_ep (st_map st))
+    end in
+  code_state (PTree.set new_ep instr (st_code st)) new_ep new_map.
 
 Definition reg_a:   ident := 1%positive.
 Definition reg_x:   ident := 2%positive.
@@ -63,34 +53,46 @@ Definition reg_mem: ident := 3%positive.
 
 Open Local Scope error_monad_scope.
 
-Definition transl_instr (instr: Seccomp.instruction) (pc: Z) (st: state) : res state :=
-  match instr with
-  | Salu_add_k k =>
-    OK (add_instr (Iop (Oaddimm k) (reg_a::nil) reg_a st.(st_ep)) st)
-  | Sret_a =>
-    OK (add_instr (Ireturn (Some reg_a)) st)
-  | _ => Error (msg "FIXME")
+Definition transl_instr (instr: Seccomp.instruction) (pc: positive)
+                        (st: state) : res state :=
+  match st, instr with
+  | code_state _ ep _, Salu_add_k k =>
+    OK (add_instr (Iop (Oaddimm k) (reg_a::nil) reg_a ep) st (Some pc))
+  | _, Sret_a =>
+    OK (add_instr (Ireturn (Some reg_a)) st (Some pc))
+  | empty_state, _ => Error (msg "No trailing ret")
+  | _, _ => Error (msg "FIXME")
   end.
 
-Fixpoint transl_code (src: Seccomp.code) (pc: Z) (st: state) : res state :=
+Fixpoint transl_code (src: Seccomp.code) (pc: positive)
+                     (st: state) : res state :=
   match src with
   | nil => OK st
   | hd::tl =>
-    do st <- transl_code tl (Zsucc pc) st;
-    do st <- transl_instr hd pc st;
-    OK (add_map pc st)
+    do st <- transl_code tl (Psucc pc) st;
+    transl_instr hd pc st
   end.
 
+
+Record fnmap: Type := mkfnmap {
+  fn: RTL.function;
+  map: PTree.t node
+}.
+
 Definition transl_function (f: Seccomp.function) : res fnmap :=
-  let st := mkstate (PTree.empty RTL.instruction) 1%positive (ZMap.init 1%positive) in
-  do st <- transl_code f 0 st;
+  do st <- transl_code f 1 empty_state;
   let sig := mksignature nil (Some Tint) in
   let stacksize := (Zmult seccomp_memwords 4) in
   (* FIXME: memset(mem, 0, sizeof(mem)) *)
-  let st := add_instr (Iop (Oaddrstack Int.zero) nil reg_mem st.(st_ep)) st in
-  let st := add_instr (Iop (Ointconst Int.zero) nil reg_x st.(st_ep)) st in
-  let st := add_instr (Iop (Ointconst Int.zero) nil reg_a st.(st_ep)) st in
-  OK (mkfnmap (RTL.mkfunction sig nil stacksize st.(st_code) st.(st_ep)) st.(st_map)).
+  do ep <- st_ep st;
+  let st := add_instr (Iop (Oaddrstack Int.zero) nil reg_mem ep) st None in
+  do ep <- st_ep st;
+  let st := add_instr (Iop (Ointconst Int.zero) nil reg_x ep) st None in
+  do ep <- st_ep st;
+  let st := add_instr (Iop (Ointconst Int.zero) nil reg_a ep) st None in
+  do ep <- st_ep st;
+  OK (mkfnmap (RTL.mkfunction sig nil stacksize (st_code st) ep)
+              (st_map st)).
 
 Local Open Scope string_scope.
 
